prove equal routine.

Cslib/Computability/Machines/MultiTapeTuring/EqualRoutine.lean
@@ -13,6 +13,8 @@ public import Cslib.Computability.Machines.MultiTapeTuring.Basic
 public import Cslib.Computability.Machines.MultiTapeTuring.ListEncoding
 public import Cslib.Computability.Machines.MultiTapeTuring.WithTapes
 
+import Mathlib.Logic.Function.Basic
+
 namespace Turing
 
 namespace Routines
@@ -20,36 +22,38 @@ namespace Routines
 --- A 3-tape Turing machine that pushes the new word "1"
 --- to the third tape if the first words on the first and second tape are the same
 --- and otherwise pushes the empty word to the third tape.
+--- If one of the first two tapes is empty, uses the empty word for comparison.
 public def eq₀ : MultiTapeTM 3 (WithSep OneTwo) where
   Λ := PUnit
   q₀ := 0
   M _ syms := sorry
 
 @[simp]
-public theorem eq₀_eval_list (w₁ w₂ : List OneTwo) (ws₁ ws₂ ws₃ : List (List OneTwo)) :
-  eq₀.eval_list [w₁ :: ws₁, w₂ :: ws₂, ws₃].get =
-    Part.some (if w₁ = w₂ then
-      [w₁ :: ws₁, w₂ :: ws₂, [.one] :: ws₃].get
+public theorem eq₀_eval_list {tapes : Fin 3 → List (List OneTwo)} :
+  eq₀.eval_list tapes =
+    Part.some (Function.update tapes 2 ((if (tapes 0).headD [] = (tapes 1).headD [] then
+      [.one]
     else
-      [w₁ :: ws₁, w₂ :: ws₂, [] :: ws₃].get) := by
+      []) :: (tapes 2))) := by
   sorry
 
-public def eq {k : ℕ} (q s t : Fin k.succ)
+public def eq {k : ℕ} (q s t : Fin k)
   (h_neq : q ≠ s := by decide) (h_neq' : q ≠ t := by decide) (h_neq'' : s ≠ t := by decide) :
-  MultiTapeTM k.succ (WithSep OneTwo) :=
-  eq₀.with_tapes #v[q, s, t] (h_le := by omega)
+  MultiTapeTM k (WithSep OneTwo) :=
+  eq₀.with_tapes [q, s, t].get (by intro x y; grind) (h_le := by omega)
 
 @[simp, grind =]
-public theorem eq_eval_list {k : ℕ} {q s t : Fin k.succ}
+public theorem eq_eval_list {k : ℕ} {q s t : Fin k}
   {h_neq : q ≠ s} {h_neq' : q ≠ t} {h_neq'' : s ≠ t}
-  {tapes : Fin k.succ → List (List OneTwo)} {h_q_nonempty : tapes q ≠ []} {h_s_nonempty : tapes s ≠ []} :
+  {tapes : Fin k → List (List OneTwo)} :
   (eq q s t (h_neq := h_neq) (h_neq' := h_neq') (h_neq'' := h_neq'')).eval_list tapes =
-    Part.some (Function.update tapes t
-      ((if (tapes q).head h_q_nonempty = (tapes s).head h_s_nonempty then
-        [.one]
-      else
-        []) :: (tapes t))) := by
-  sorry
+    Part.some (Function.update tapes t ((if (tapes q).headD [] = (tapes s).headD [] then
+      [.one]
+    else
+      []) :: (tapes t))) := by
+  have h_inj : [q, s, t].get.Injective := by intro x y; grind
+  simp [eq]
+  grind
 
 end Routines
 
