Cslib/Computability/Machines/MultiTapeTuring/PopRoutine.lean
@@ -29,33 +29,19 @@ public def pop₁ : MultiTapeTM 1 (WithSep α) where
   M _ syms := sorry
 
 @[simp]
-public lemma pop₁_eval_list {w : List α} {ls : List (List α)} :
-  pop₁.eval_list [w :: ls].get = .some [ls].get := by
+public lemma pop₁_eval_list {tapes : Fin 1 → List (List α)} :
+  pop₁.eval_list tapes = .some (Function.update tapes 0 (tapes 0).tail) := by
   sorry
 
 public def pop {k : ℕ} (i : Fin k.succ) : MultiTapeTM k.succ (WithSep α) :=
-  pop₁.with_tapes #v[i] (h_le := by omega)
+  pop₁.with_tapes [i].get (by intro x y; grind) (h_le := by omega)
 
 @[simp, grind =]
 public theorem pop_eval_list {k : ℕ} {i : Fin k.succ}
-  {tapes : Fin k.succ → List (List α)}
-  {h_not_empty : tapes i ≠ []} :
+  {tapes : Fin k.succ → List (List α)} :
   (pop i).eval_list tapes = .some (Function.update tapes i (tapes i).tail) := by
-  sorry
-
-public def pop' {k aux : ℕ} (i : ℕ) (h_i_lt : i < k := by decide) :
-    MultiTapeTMWithAuxTapes k aux (WithSep α) :=
-  (pop₁.allocate_aux_tapes aux).with_tapes #v[⟨i, h_i_lt⟩]
-    (h_le_k := by omega)
-    (h_le_aux := by rfl)
-
-@[simp, grind =]
-public theorem pop'_eval_list {k aux i : ℕ} {h_i_lt : i < k}
-  {tapes : Fin k → List (List α)}
-  {h_not_empty : tapes ⟨i, h_i_lt⟩ ≠ []} :
-  (pop' (aux := aux) i h_i_lt).eval_list_aux tapes = .some
-    (Function.update tapes ⟨i, h_i_lt⟩ (tapes ⟨i, h_i_lt⟩).tail) := by
-  sorry
+  simp [pop]
+  grind
 
 end Routines
 
