Cslib/Computability/Machines/MultiTapeTuring/PushRoutine.lean
@@ -13,9 +13,6 @@ public import Cslib.Computability.Machines.MultiTapeTuring.Basic
 public import Cslib.Computability.Machines.MultiTapeTuring.ListEncoding
 public import Cslib.Computability.Machines.MultiTapeTuring.WithTapes
 
--- TODO create a "common file"
-import Cslib.Computability.Machines.SingleTapeTuring.Basic
-
 namespace Turing
 
 namespace Routines
@@ -28,25 +25,27 @@ public def push₁ (w : List α) : MultiTapeTM 1 (WithSep α) where
   M _ syms := sorry
 
 @[simp]
-public lemma push₁_eval_list {w : List α} {ls : List (List α)} :
-  (push₁ w).eval_list [ls].get = .some [w :: ls].get := by
+public lemma push₁_eval_list {w : List α} {tapes : Fin 1 → List (List α)} :
+  (push₁ w).eval_list tapes = .some (Function.update tapes 0 (w :: (tapes 0))) := by
   sorry
 
 public def push {k : ℕ} (i : Fin k.succ) (w : List α) : MultiTapeTM k.succ (WithSep α) :=
-  (push₁ w).with_tapes #v[i] (h_le := by omega)
+  (push₁ w).with_tapes [i].get (by intro x y; grind) (h_le := by omega)
 
 @[simp, grind =]
-public theorem push_eval_list {k : ℕ} (i : Fin k.succ) (w : List α) (tapes : Fin k.succ → List (List α)) :
+public theorem push_eval_list {k : ℕ}
+  {i : Fin k.succ} {w : List α} {tapes : Fin k.succ → List (List α)} :
   (push i w).eval_list tapes =
     .some (Function.update tapes i (w :: (tapes i))) := by
-  sorry
+  simp [push]
+  grind
 
-public lemma push₁_evalWithStats_list {w : List α} {ls : List (List α)} :
-  (push₁ w).evalWithStats_list #v[ls].get =
-    .some (
-      [w :: ls].get,
-      [⟨-w.length - 1, 0, -w.length - 1, by omega⟩].get) := by
-  sorry
+-- public lemma push₁_evalWithStats_list {w : List α} {ls : List (List α)} :
+--   (push₁ w).evalWithStats_list #v[ls].get =
+--     .some (
+--       [w :: ls].get,
+--       [⟨-w.length - 1, 0, -w.length - 1, by omega⟩].get) := by
+--   sorry
 
 end Routines
 
