Cslib/Computability/Machines/MultiTapeTuring/GraphReachability.lean
@@ -71,31 +71,4 @@ def reachable(a, b, t, r):
 -/
 
 
-
-namespace Routines
-
-variable [Inhabited α] [Fintype α]
-
-public def copy : MultiTapeTM 2 (WithSep α) where
-  Λ := PUnit
-  q₀ := 0
-  M _ syms := sorry
-
-@[simp]
-public lemma copy_eval_list {w : List α} {ls₁ ls₂ : List (List α)} :
-  copy.eval_list [w :: ls₁, ls₂].get = Part.some [w :: ls₁, w :: ls₂].get := by
-  sorry
-
-public lemma copy_evalWithStats {w : List α} {ls₁ ls₂ : List (List α)} :
-  copy.evalWithStats_list #v[w :: ls₁, ls₂].get =
-    .some (
-      [w :: ls₁, w :: ls₂].get,
-      [⟨-1, w.length, 0, by omega⟩, ⟨-w.length - 2, 0, -w.length - 1, by omega⟩].get) := by
-  sorry
-
--- TODO at some point, we might not want exact stats but rather an upper bound.
--- Can this be made compatible with using equality?
-
-end Routines
-
 end Turing
